Sometimes if we are asked to integrate a function containing a fraction,
we can make the integration easier by changing the fraction into partial
fractions.

eg:
$$\mathrm{I} = \int \frac {1}{\mathrm{x}^2 + 3 \mathrm{x} + 2} \mathrm{dx}$$
$$= \int \frac {1}{ \mathrm{(x + 2)(x + 1)}}\mathrm{dx}$$
$$= \int \left ( \frac {-1}{\mathrm{x}+2} + \frac {1}{\mathrm{x} + 1} \right ) \mathrm{dx}$$
$$= - \ln ( \mathrm{x} + 2) + \ln ( \mathrm{x} + 1) + \mathrm{C}$$
$$= \ln \left ( \frac{\mathrm{x} + 1}{\mathrm{x}+2} \right ) + \mathrm{C}$$
