This is the method for solving any cubic equation:

Say we have $ {ax} ^3 + {bx} ^2 + {cx + d} = 0 $

Then we define a new variable, y, and set $ {y = x} + 
\frac{{b}}{3 {a}} $

So $ {x = y} - \frac{{b}}{3 {a}}, $

and the equation becomes: $ {ay} ^3 
+ ({c} - \frac{{b}^2}{3 {a}} ) {y} 
+ \frac{2 {b}^3}{27 {a} ^2} - \frac{{bc}}{3 {a}} 
+ {d} = 0 $

which we can write as: $ {y}^3 + {py + q} = 0 $

by dividing by a and defining p and q appropriately.

Next define two new variables u and v, with $ {uv} = \frac{{p}}{3}, $

and $ {y = u - v} . $

So then: $ {u}^3 - {v}^3 + {q} = 0. $

But $ {v} = \frac{{p}}{3 {u}}, $

so this becomes: $ ( {u}^3 ) ^2 + {qu}^3 - \frac{{p} ^3}{27} = 0 $

which is a quadratic equation in $ {u}^3 . $

We can solve this to find $ {u}^3 , $ so we can find u, and then v,
because $ {v} = \frac{{p}}{3 {u}} . $

Then we can find y, because $ {y = u - v}, $

and finally we can find x: $${x} = 
 ^3 \sqrt {\frac{- {q} + \sqrt{{q}^2 + \frac{4}{27} {p} ^3 } } {2}}
+  ^3 \sqrt {\frac{- {q} - \sqrt{{q}^2 + \frac{4}{27} {p} ^3 } } {2} } 
- \frac{{b}}{3 {a}}$$

with $ {p} = \frac{{c}}{{a}} 
- \frac{{b}^2}{3 {a} ^2 }, 
{q} = \frac{2 {b}^3}{27 {a}^3}
- \frac{{bc}}{3 {a}^2} 
+ \frac{{d}}{{a}}. $
