If we write the elliptic integral of the first kind in this form:
$$\mathrm{u} = \int _{0} ^{\mathrm{x}} \frac{\mathrm{dt}} 
{ \sqrt{((1- \mathrm{t}^2 ) ( 1 - \mathrm{k}^2 \mathrm{t}^2 )) } } ,$$
then the elliptic functions sn, cn and dn can be defined as:
$$\mathrm{x = sn(u)} ,$$
$$\sqrt{ 1 - \mathrm{x} ^2 } = \mathrm{cn(u)} ,$$
$$\sqrt{ 1 - \mathrm{k}^2 \mathrm{x}^2 } = \mathrm{dn(u)} .$$

(This is analogous to defining the circular functions in terms of the
integral $ \mathrm{u} = \int _{0} ^{\mathrm{x}} \frac{\mathrm{dt}}
{\sqrt{1-\mathrm{t}^2}} , $ x=sin(u). )
